hol/cake_sem/p4_exec_sem_cake_exportScript.sml
@@ -1,0 +1,500 @@
+open HolKernel boolLib Parse bossLib;
+
+val _ = new_theory "p4_exec_sem_cake_export";
+
+open p4Theory p4_auxTheory p4_coreTheory p4_v1modelTheory;
+open p4_exec_sem_cakeTheory p4_arch_cakeTheory;
+
+(* CakeML: *)
+open preamble ml_translatorLib ml_translatorTheory ml_progLib basisProgTheory mlmapTheory basisFunctionsLib
+     astPP comparisonTheory;
+
+intLib.deprecate_int();
+val _ = (max_print_depth := 100);
+
+val _ = translation_extends "basisProg";
+
+val _ = ml_prog_update (open_module "p4_exec_sem_cake");
+
+(** Expression semantics **)
+
+val _ = translate numposrepTheory.l2n_def;
+val _ = translate bitstringTheory.bitify_def;
+val _ = translate bitstringTheory.v2n_def;
+Theorem l2n_side_thm:
+!n l. l2n_side n l <=> (l <> [] ==> n <> 0)
+Proof
+strip_tac \\
+Induct \\ (
+ rpt strip_tac \\
+ ONCE_REWRITE_TAC[theorem "l2n_side_def"] \\
+ gs[]
+) \\
+Cases_on ‘l’ \\ (
+ gs[]
+)
+QED
+val _ = update_precondition l2n_side_thm;
+Theorem v2n_side:
+!v1. v2n_side v1
+Proof
+gs[definition "v2n_side_def", l2n_side_thm, bitstringTheory.bitify_def]
+QED
+val _ = update_precondition v2n_side;
+
+val _ = translate numposrepTheory.n2l_def;
+val _ = translate bitstringTheory.boolify_def;
+val _ = translate bitstringTheory.n2v_def;
+Theorem n2l_side_thm:
+!n m. n2l_side n m <=> n <> 0
+Proof
+strip_tac \\
+completeInduct_on ‘m’ \\
+rpt strip_tac \\
+ONCE_REWRITE_TAC[theorem "n2l_side_def"] \\
+gs[]
+QED
+val _ = update_precondition n2l_side_thm;
+Theorem n2v_side:
+!v. n2v_side v
+Proof
+gs[definition "n2v_side_def", n2l_side_thm]
+QED
+val _ = update_precondition n2v_side;
+
+val _ = translate find_topmost_map'_def;
+val _ = translate lookup_map'_def;
+val _ = translate lookup_vexp2'_def;
+val _ = translate is_v'_def;
+val _ = translate e_exec_acc'_def;
+val _ = translate INDEX_FIND_def;
+val _ = translate is_const'_def;
+val _ = translate unred_mem'_def;
+val _ = translate unred_mem_index'_def;
+val _ = translate MAP_SND_def;
+val _ = translate v_of_e'_def;
+val _ = translate vl_of_el'_def;
+val _ = translate MAP_FST_def;
+val _ = translate oEL_def;
+val _ = translate listTheory.LUPDATE_DEF;
+
+(* Function call *)
+val _ = translate lookup_funn_sig_body'_def;
+val _ = translate is_d_out_def;
+val _ = translate get_lval_of_e'_def;
+val _ = translate is_e_lval'_def;
+val _ = translate is_arg_red'_def;
+val _ = translate find_unred_arg'_def;
+val _ = translate unred_arg_index'_def;
+val _ = translate listTheory.FOLDL;
+val _ = translate find_topmost_map'_def;
+val _ = translate lookup_map'_def;
+val _ = translate lookup_v'_def;
+val _ = translate acc_f_def;
+
+val _ = translate rich_listTheory.SEG;
+Theorem seg_side_thm:
+!len start l. seg_side len start l <=> (len <> 0 ==> (start + len <= LENGTH l))
+Proof
+strip_tac \\
+completeInduct_on ‘len’ \\
+completeInduct_on ‘start’ \\
+rpt strip_tac \\
+ONCE_REWRITE_TAC[theorem "seg_side_def"] \\
+gs[] \\
+eq_tac >- (
+ rpt strip_tac >- (
+  res_tac \\
+  gs[]
+ ) \\
+ gs[] \\
+ qpat_x_assum ‘!m. m < SUC x4 ==>
+               !l'. seg_side (SUC x3) m l' <=> m + SUC x3 <= LENGTH l'’
+              (fn thm => ASSUME_TAC $ Q.SPEC ‘x4’ thm) \\
+ gs[arithmeticTheory.SUC_ONE_ADD]
+) \\
+rpt strip_tac \\ (
+ gs[]
+) >- (
+ Cases_on ‘len’ \\ Cases_on ‘start’ \\ (
+  gs[]
+ ) >- (
+  Cases_on ‘l’ \\ (
+   gs[]
+  )
+ ) \\
+ Cases_on ‘l’ \\ (
+  gs[]
+ )
+) \\
+qpat_x_assum ‘!m. m < SUC x10 ==>
+              !l'. seg_side (SUC x13) m l' <=> m + SUC x13 <= LENGTH l'’
+             (fn thm => ASSUME_TAC $ Q.SPEC ‘x10’ thm) \\
+gvs[] \\
+gs[arithmeticTheory.SUC_ONE_ADD]
+QED
+val _ = update_precondition seg_side_thm;
+val _ = translate bitv_bitslice_def;
+val _ = translate slice'_def;
+Theorem slice'_side:
+!v1 v2 v3. slice'_side v1 v2 v3
+Proof
+simp[Once $ definition "slice'_side_def"] \\
+simp[Once $ definition "bitv_bitslice_side_def"]
+QED
+val _ = update_precondition slice'_side;
+val _ = translate slice_lval'_def;
+val _ = translate lookup_lval'_def;
+
+val _ = translate is_d_in_def;
+val _ = translate bitstringTheory.extend_def;
+val _ = translate init_out_v_cake_def;
+val _ = translate one_arg_val_for_newscope'_def;
+val _ = translate AFUPDKEY_def;
+val _ = translate AUPDATE_def;
+val _ = translate update_arg_for_newscope'_def;
+val _ = translate all_arg_update_for_newscope'_def;
+val _ = translate copyin'_def;
+
+(* Cast *)
+val _ = translate bitstringTheory.zero_extend_def;
+val _ = translate listTheory.DROP_def;
+val _ = translate bitstringTheory.fixwidth_def;
+val _ = translate bool_cast_def;
+val _ = translate bitv_cast_def;
+val _ = translate oHD_def;
+val _ = translate to_bool_cast_exec_def;
+val _ = translate cast_exec_def;
+val _ = translate e_exec_cast'_def;
+
+(* Unops *)
+val _ = translate bitv_1comp_def;
+val _ = translate bitv_2comp_def;
+val _ = translate unop_exec'_def;
+val _ = translate e_exec_unop'_def;
+
+(* Select *)
+val _ = translate bitv_ls_def;
+val _ = translate bitv_hs_def;
+val _ = translate bitv_lo_def;
+val _ = translate bitv_hi_def;
+val _ = translate rich_listTheory.AND_EL_DEF;
+val _ = translate bit_eq_def;
+val _ = translate bitv_eq_def;
+val _ = translate bitv_neq_def;
+val _ = translate get_bitv_binpred'_def;
+val _ = translate bitv_binpred'_def;
+val _ = translate p4_match_range'_def;
+val _ = translate bitv_mul_def;
+val _ = translate bitv_div_def;
+val _ = translate bitv_mod_def;
+val _ = translate bitv_add_def;
+val _ = translate bitv_sub_def;
+
+val _ = translate band'_def;
+val _ = translate bitv_and_def;
+val _ = translate bor'_def;
+val _ = translate bitv_or_def;
+val _ = translate bitstringTheory.bitwise_def;
+val _ = translate bitstringTheory.bxor_def;
+val _ = translate bitv_xor_def;
+
+val _ = translate rich_listTheory.REPLICATE;
+val _ = translate bitv_saturate_add_def;
+val _ = translate bitv_saturate_sub_def;
+val _ = translate bitv_lsl_bv_def;
+val _ = translate rich_listTheory.TAKE;
+val _ = translate bitv_lsr_bv_def;
+Theorem take_1_side_thm:
+!n l. take_1_side n l <=> n <= LENGTH l
+Proof
+Induct \\ (
+ simp[Once $ theorem "take_1_side_def"]
+) \\
+rpt strip_tac \\
+Cases_on ‘l’ \\ (
+ gs[]
+)
+QED
+val _ = update_precondition take_1_side_thm;
+Theorem bitv_lsr_bv_side:
+!v1 v2 l. bitv_lsr_bv_side v1 v2 l
+Proof
+simp[Once $ definition "bitv_lsr_bv_side_def", take_1_side_thm]
+QED
+val _ = update_precondition bitv_lsr_bv_side;
+val _ = translate p4Theory.binop2num_thm;
+val _ = translate p4Theory.binop_CASE;
+val _ = translate get_bitv_binop'_def;
+val _ = translate bitv_binop'_def;
+val _ = translate p4_match_mask'_def;
+val _ = translate match'_def;
+val _ = translate match_all'_def;
+val _ = translate match_all_first'_def;
+val _ = translate match_all_first_def;
+val _ = translate e_exec_select'_def;
+
+(* Binops *)
+val _ = translate is_short_circuitable_def;
+val _ = translate e_exec_short_circuit'_def;
+val _ = translate bitv_bl_binop_def;
+val _ = translate bitstringTheory.shiftl_def;
+val _ = translate bitstringTheory.shiftr_def;
+val _ = translate binop_exec'_def;
+val _ = translate e_exec_binop'_def;
+    
+(* Concatenation *)
+val _ = translate bitv_concat_def;
+val _ = translate e_exec_concat'_def;
+val _ = translate is_v_bit'_def;
+
+(* Slicing *)
+val _ = translate e_exec_slice'_def;
+
+(* The whole expression-level semantics: *)
+val _ = translate e_exec'_def;
+
+(** Statement semantics **)
+
+(* Assignment *)
+val _ = translate lookup_out'_def;
+val _ = translate listTheory.INDEX_OF_def;
+val _ = translate replace_bits_def;
+Theorem replace_bits_side:
+!bitv1 bitv2 hi lo. replace_bits_side bitv1 bitv2 hi lo
+Proof
+simp[Once $ definition "replace_bits_side_def"]
+QED
+val _ = update_precondition replace_bits_side;
+val _ = translate assign_to_slice'_def;
+val _ = translate assign'_def;
+val _ = translate stmt_exec_ass'_def;
+val _ = translate oDROP_def;
+val _ = translate oTAKE_def;
+val _ = translate separate_def;
+val _ = translate get_e_ctx_def;
+
+(* Conditional *)
+val _ = translate is_v_bool'_def;
+val _ = translate stmt_exec_cond'_def;
+
+(* Block *)
+val _ = translate init_v_from_tau_cake_def;
+val _ = translate declare_list_in_fresh_scope'_def;
+
+(* Return *)
+val _ = translate get_v'_def;
+
+(* Sequence *)
+val _ = translate is_empty'_def;
+
+(* Transition *)
+val _ = translate is_v_str'_def;
+val _ = translate stmt_exec_trans'_def;
+
+(* Apply *)
+val _ = translate index_not_const'_def;
+val _ = translate is_consts_exec'_def;
+
+(* Extern *)
+val _ = translate lookup_ext_fun'_def;
+
+val _ = translate stmt_exec'_def;
+
+(** Frame semantics **)
+
+val _ = translate scopes_to_pass'_def;
+val _ = translate map_to_pass'_def;
+val _ = translate tbl_to_pass'_def;
+val _ = translate scopes_to_retrieve'_def;
+
+val _ = translate is_d_none_in_def;
+val _ = translate update_return_frame'_def;
+val _ = translate copyout'_def;
+Theorem copyout'_side:
+!xlist dlist gsl ss ss_curr. copyout'_side xlist dlist gsl ss ss_curr
+Proof
+simp[Once $ definition "copyout'_side_def"] \\
+rpt strip_tac >- (
+ gs[oTAKE_TAKE]
+) \\
+gs[oDROP_DROP]
+QED
+val _ = update_precondition copyout'_side;
+val _ = translate frames_exec'_def;
+
+(** Arch semantics **)
+
+val _ = translate lookup_block_body_def;
+val _ = translate oLASTN_def;
+val _ = translate declare_list_in_scope'_def;
+val _ = translate AUPDATE_LIST_def;
+val _ = translate var_star_updates_of_func_map'_def;
+val _ = translate var_star_updates_of_ext_map'_def;
+val _ = translate initialise_var_stars'_def;
+val _ = translate state_fin_exec_def;
+val _ = translate set_fin_status_def;
+
+val _ = translate arch_exec'_def;
+
+val _ = translate arch_multi_exec'_def;
+
+(** Core arch implementation **)
+
+val _ = translate header_is_valid'_def;
+
+val _ = translate header_set_valid'_def;
+
+val _ = translate header_set_invalid'_def;
+
+(* TODO: Below two functions are used for wrapper *)
+Definition p4_append_input_list'_def:
+ (p4_append_input_list' [] (astate:'a astate') = astate) /\
+ (p4_append_input_list' (h::t) astate =
+   case astate of
+   | (aenv, gscope, afl, status) =>
+    p4_append_input_list' t
+     (case aenv of
+      | (ab_index, inputl, outputl, ascope) => 
+       ((ab_index, inputl++[h], outputl, ascope), gscope, afl, status)))
+End
+
+Definition p4_get_output_list_def:
+ p4_get_output_list (((i, io_list, io_list', ascope), g_scope_list, arch_frame_list, status):'a astate') =
+  io_list'
+End
+
+val _ = translate p4_append_input_list'_def;
+val _ = translate p4_get_output_list_def;
+
+(* Common extern functions: *)
+
+val _ = translate oTAKE_DROP_def;
+val _ = translate v2w16s'''_def;
+val _ = translate header_entries2v_def;
+val _ = translate v2w16s''_def;
+val _ = translate p4_arch_cakeTheory.get_checksum_incr''_def;
+
+val _ = translate add_with_carry'_def;
+val _ = translate add_ones_complement'_def;
+val _ = translate compute_checksum16_inner_def;
+val _ = translate all_lists_length_16_def;
+val _ = translate compute_checksum16_def;
+Theorem compute_checksum16_side:
+!v1. compute_checksum16_side v1
+Proof
+simp[Once $ definition "compute_checksum16_side_def"] \\
+Induct >- (
+ simp[Once $ theorem "compute_checksum16_inner_side_def", all_lists_length_16_def]
+) \\
+rpt strip_tac \\
+gs[all_lists_length_16_def, Once $ theorem "compute_checksum16_inner_side_def"] \\
+Cases_on ‘v1’ >- (
+ gs[theorem "compute_checksum16_inner_side_def",
+    compute_checksum16_inner_def, Once $ definition "add_ones_complement'_side_def",
+    Once $ definition "add_with_carry'_side_def"] \\
+ rpt strip_tac \\ (
+  gs[bitstringTheory.fixwidth_def, AllCaseEqs(), bitstringTheory.zero_extend_def,
+     listTheory.PAD_LEFT]
+ ) 
+) \\
+qpat_x_assum ‘!x2 x1. _’ (fn thm => ASSUME_TAC $ Q.SPECL [‘h'’, ‘t’] thm) \\
+simp[Once $ theorem "compute_checksum16_inner_side_def",
+     Once $ definition "add_ones_complement'_side_def",
+     Once $ definition "add_with_carry'_side_def"] \\
+rpt strip_tac >- (
+ gs[]
+) >- (
+ gs[compute_checksum16_inner_def, add_ones_complement'_def, add_with_carry'_def,
+    AllCaseEqs(), bitstringTheory.fixwidth_def, AllCaseEqs(),
+    bitstringTheory.zero_extend_def, listTheory.PAD_LEFT]
+) >- (
+ gs[]
+) >- (
+ gs[bitstringTheory.fixwidth_def, AllCaseEqs(), bitstringTheory.zero_extend_def,
+    listTheory.PAD_LEFT]
+) \\
+simp[Once $ theorem "compute_checksum16_inner_side_def"]
+QED
+val _ = update_precondition compute_checksum16_side;
+
+(** V1Model arch implementation **)
+
+(* Architectural functions: *)
+
+val _ = translate v_map_to_scope'_def;
+val _ = translate oCONS_def;
+val _ = translate scope_to_vmap'_def;
+val _ = translate v1model_ascope_update'_def;
+val _ = translate v1model_postparser'_def;
+
+val _ = translate v1model_input_f'_def;
+
+val _ = translate v1model_is_drop_port_def;
+val _ = translate v1model_lookup_obj_def;
+val _ = translate v1model_output_f'_def;
+
+val _ = translate v1model_reduce_nonout'_def;
+val _ = translate v1model_copyin_pbl'_def;
+
+val _ = translate copyout_pbl_gen'_def;
+val _ = translate v1model_copyout_pbl'_def;
+
+val _ = translate FOLDL_MATCH_alt_def;
+val _ = translate FOLDL_MATCH_def;
+val _ = translate listTheory.LIST_TO_SET_DEF;
+val _ = translate boolTheory.IN_DEF;
+val _ = translate v1model_apply_table_f'_def;
+
+(* Extern implementations: *)
+
+val _ = translate v1model_mark_to_drop'_def;
+
+val _ = translate v1model_ascope_update_v_map'_def;
+val _ = translate verify_gen'_def;
+val _ = translate v1model_verify'_def;
+
+val _ = translate v1model_verify_checksum'_def;
+
+val _ = translate v1model_update_checksum'_def;
+
+val _ = translate lookup_lval_header'_def;
+val _ = translate lookup_ascope_gen_def;
+val _ = translate size_in_bits_def;
+val _ = translate set_bool_def;
+val _ = translate set_bit_def;
+val _ = translate set_fields_def;
+val _ = translate set_header_def;
+val _ = translate update_ascope_gen_def;
+val _ = translate packet_in_extract_gen'_def;
+val _ = translate v1model_ascope_lookup'_def;
+val _ = translate v1model_packet_in_extract'_def;
+
+val _ = translate set_struct_def;
+val _ = translate set_v_def;
+val _ = translate packet_in_lookahead_gen'_def;
+val _ = translate v1model_packet_in_lookahead'_def;
+
+val _ = translate lookup_lval_bit32'_def;
+val _ = translate packet_in_advance_gen'_def;
+val _ = translate v1model_packet_in_advance'_def;
+
+val _ = translate flatten_v_l_def;
+val _ = translate packet_out_emit_gen'_def;
+val _ = translate v1model_packet_out_emit'_def;
+
+(* TODO: The below is defined in terms of functions that uses ARB... *)
+(*
+val _ = translate v1model_register_construct_inner_def;
+val _ = translate register_construct_def;
+
+val _ = translate v1model_register_read_inner_def;
+val _ = translate register_read'_def;
+*)
+
+val _ = translate v1model_register_write_inner_def;
+val _ = translate register_write'_def;
+
+val _ = ml_prog_update (close_module NONE);
+
+val _ = export_theory ();
